src/lib/updates.v
@@ -15,8 +15,22 @@ From iris.prelude Require Import options.
 (* Infix "~~>:{  t  }" := (cmra_updateP t) (at level 70). *)
 
 
+(* ∃ x' x1' x2', x' ≡{k}≡ x1' ⋅ x2' /\ x1' ≡{k}≡ t x1' *)
+(*                                             /\ (∃ x2, x ≡{k}≡ x2 ⋅ x2' /\ (∀ x3 x2'' yf', x2 ≡{k}≡ t x3 -> x2' ≡{k}≡ t x2'' -> yf ≡{k}≡ t yf' -> *)
+(*                                                                                         ✓{k} (x3 ⋅ x2'' ⋅ yf') -> ✓{k} (x1' ⋅ x2'' ⋅ yf'))) *)
+(*                                             /\ ✓{k} (x' ⋅ yf) *)
+(*               /\ Q k x' *)
+
+
+Definition upd_img_rel {A : cmra} (t : A → A) `{!CmraMorphism t} (x1 y1 y2 : A) (mz : option A) (k : nat) :=
+  (∀ x1' y2' mz', x1 ≡{k}≡ t x1' -> y2 ≡{k}≡ t y2' -> (from_option (λ a, mz' ≡{k}≡ Some (t a)) (mz' ≡{k}≡ None) mz) ->
+                  ✓{k} (x1' ⋅ y2' ⋅? mz') -> ✓{k} (y1 ⋅ y2' ⋅? mz')).
+Definition upd_rel {A : cmra} (t : A → A) `{!CmraMorphism t} (x : A) (y : A) (k : nat) (mz : option A) :=
+  ∃ (y1 y2 x1: A), (y ≡{k}≡ y1 ⋅ y2 /\ t y1 ≡{k}≡ y1 /\ x ≡{k}≡ x1 ⋅ y2) /\ upd_img_rel t x1 y1 y2 mz k.
+  
+
 Definition cmra_updateP {A : cmra} (t : A → A) `{!CmraMorphism t} (x : A) (P : A → Prop) := ∀ n (mz : option A),
-  ✓{n} (x ⋅? mz) /\ t x ≡ x -> ∃ y, P (y) /\ ✓{n} (y ⋅? mz) ∧ t y ≡ y.
+    ✓{n} (x ⋅? mz) -> ∃ y, P (y) /\ ✓{n} (y ⋅? mz) /\ upd_rel t x y n mz.
 Global Instance: Params (@cmra_updateP) 1 := {}.
 Global Instance: Params (@cmra_updateP) 3 := {}.
 Infix "~~>:{  t  }" := (cmra_updateP t) (at level 70).
@@ -28,75 +42,105 @@ Infix "~~>:{  t  }" := (cmra_updateP t) (at level 70).
 (* Global Instance: Params (@cmra_update) 3 := {}. *)
 
 Definition cmra_update {A : cmra} (t : A → A) `{!CmraMorphism t} (x y : A) := ∀ n mz,
-  ✓{n} (x ⋅? mz) /\ t x ≡ x -> ✓{n} (y ⋅? mz) /\ t y ≡ y.
+  ✓{n} (x ⋅? mz) -> ✓{n} (y ⋅? mz) /\ upd_rel t x y n mz.
 Infix "~~>{  t  }" := (cmra_update t) (at level 70).
 Global Instance: Params (@cmra_update) 1 := {}.
 Global Instance: Params (@cmra_update) 3 := {}.
 
 
+
+(* Lemma equiv_Some_l {A : cmra} (c : A) (mz : option A) : *)
+(*   Some c ≡ mz -> ∃ (c' : A), mz = Some c' /\ c' ≡ c. *)
+(* Proof. *)
+(*   intros Hc. *)
+(*   inversion Hc;subst;eauto. *)
+(* Qed. *)
+
+Class GenTransContractive {A : cmra} (f : A -> A) := {
+    gen_trans_contr n a : (f a ≼{n} a)
+}.
+
 Section updates.
-Context {A : cmra} (t : A -> A) `{morph: !CmraMorphism t}.
+Context {A : ucmra} (t : A -> A) `{morph: !CmraMorphism t} `{!GenTransContractive t}.
 Implicit Types x y : A.
+
+Global Instance upd_img_rel_proper :
+  Proper ((≡) ==> (≡) ==> (≡) ==> (≡) ==> (=) ==> iff) (@upd_img_rel A t morph).
+Proof.
+  intros ??? y1 y2 Hy ??? mz mz' Hmz ???;subst.
+  rewrite /upd_img_rel. split=> Hyp???????;[rewrite -Hy|rewrite Hy]; eapply Hyp;eauto;
+  destruct mz;simpl;inversion Hmz;subst;simpl in *;setoid_subst;auto.
+Qed.
+  
+Global Instance upd_rel_proper :
+  Proper ((≡) ==> (≡) ==> (=) ==> (≡) ==> iff) (@upd_rel A t morph).
+Proof.
+  intros x x' Hx y y' Hy n1 n2 Heq mz mz' Hmz;subst.
+  split=> [[x1[x2[x3[HH Hyp]]]]|[x1[x2[x3[HH Hyp]]]]]; exists x1,x2,x3;split;[rewrite -Hx -Hy//| |rewrite Hx Hy//|];
+  (intros ???????; eapply Hyp;eauto;
+   destruct mz';simpl;[apply Some_equiv_eq in Hmz as [c' [-> Hc']]|inversion Hmz;subst];simpl in *;auto);[rewrite Hc'//|rewrite -Hc'//].
+Qed.
 
 Global Instance cmra_updateP_proper :
   Proper ((≡) ==> pointwise_relation _ iff ==> iff) (@cmra_updateP A t morph).
 Proof.
   rewrite /pointwise_relation /cmra_updateP=> x x' Hx P P' HP;
-    split=> ? n mz; setoid_subst; naive_solver.
+    split=> Hyp n mz;[erewrite <- Hx|erewrite Hx];intros HH;
+    apply Hyp in HH as [y [??]];exists y; setoid_subst; naive_solver.
 Qed.
 Global Instance cmra_update_proper :
   Proper ((≡) ==> (≡) ==> iff) (@cmra_update A t morph).
 Proof.
   rewrite /cmra_update=> x x' Hx y y' Hy; split=> BB n mz E; setoid_subst;auto.
 Qed.
-
+  
 Lemma cmra_update_updateP x y : x ~~>{t} y ↔ x ~~>:{t} (y =.).
 Proof. split=> Hup n z HH; eauto; destruct (Hup n z) as (?&<-&?&?);auto. Qed.
 Lemma cmra_update_updateP' x y : x ~~>{t} y ↔ x ~~>:{t} (y ≡.).
 Proof. split=> Hup n z ?; eauto; destruct (Hup n z) as (?&<-&?);auto. Qed.
-Lemma cmra_updateP_id (P : A → Prop) x : P (x) -> x ~~>:{t} P.
-Proof. intros Heq n mz [? ?]; eauto. Qed.
-Lemma cmra_updateP_compose (P Q : A → Prop) x :
-  x ~~>:{t} P → (∀ y, P y -> t y ≡ y -> y ~~>:{t} Q) → x ~~>:{t} Q.
-Proof. intros Hx Hy n mz ?. destruct (Hx n mz) as (y&HP&Heq&?); naive_solver. Qed.
-Lemma cmra_updateP_compose_l (Q : A → Prop) x y : x ~~>{t} y → y ~~>:{t} Q → x ~~>:{t} Q.
-Proof.
-  rewrite cmra_update_updateP.
-  intros Ht Hcond ???. edestruct Ht as [? [Heq [B Hequiv]]];eauto.
-  rewrite -Heq in B. subst. edestruct Hcond as (?&?&?&?);[rewrite Hequiv;eauto|];eauto. Qed.
-Lemma cmra_updateP_weaken (P Q : A → Prop) x :
-  x ~~>:{t} P → (∀ y, P y → Q y) → x ~~>:{t} Q.
-Proof. eauto using cmra_updateP_compose, cmra_updateP_id. Qed.
+(* Lemma cmra_updateP_id (P : A → Prop) x : P (x) -> x ~~>:{t} P. *)
+(* Proof. intros Heq n mz ?; eauto. Qed. *)
+(* Lemma cmra_updateP_compose (P Q : A → Prop) x : *)
+(*   x ~~>:{t} P → (∀ y, P y -> t y ≡ y -> y ~~>:{t} Q) → x ~~>:{t} Q. *)
+(* Proof. intros Hx Hy n mz ?. destruct (Hx n mz) as (y&HP&Heq&?); naive_solver. Qed. *)
+(* Lemma cmra_updateP_compose_l (Q : A → Prop) x y : x ~~>{t} y → y ~~>:{t} Q → x ~~>:{t} Q. *)
+(* Proof. *)
+(*   rewrite cmra_update_updateP. *)
+(*   intros Ht Hcond ???. edestruct Ht as [? [Heq [B Hequiv]]];eauto. *)
+(*   rewrite -Heq in B. subst. edestruct Hcond as (?&?&?&?);[rewrite Hequiv;eauto|];eauto. Qed. *)
+(* Lemma cmra_updateP_weaken (P Q : A → Prop) x : *)
+(*   x ~~>:{t} P → (∀ y, P y → Q y) → x ~~>:{t} Q. *)
+(* Proof. eauto using cmra_updateP_compose, cmra_updateP_id. Qed. *)
 
-Lemma cmra_update_exclusive `{!Exclusive x} y:
-  ✓ y -> t y ≡ y -> x ~~>{t} y.
-Proof. move=>???[z|] =>[[/exclusiveN_l[] ?]|[? ?]];simpl. split;auto.
-       by apply cmra_valid_validN. Qed.
+(* Lemma cmra_update_exclusive `{!Exclusive x} y: *)
+(*   ✓ y -> t y ≡ y -> x ~~>{t} y. *)
+(* Proof. move=>???[z|] =>[[/exclusiveN_l[] ?]|[? ?]];simpl. split;auto. *)
+(*        by apply cmra_valid_validN. Qed. *)
 
-(** Updates form a preorder. *)
-(** We set this rewrite relation's cost above the stdlib's
-  ([impl], [iff], [eq], ...) and [≡] but below [⊑].
-  [eq] (at 100) < [≡] (at 150) < [cmra_update] (at 170) < [⊑] (at 200) *)
-Global Instance cmra_update_rewrite_relation :
-  RewriteRelation (@cmra_update A t morph) | 170 := {}.
-Global Instance cmra_update_preorder : PreOrder (@cmra_update A t morph).
-Proof.
-  split.
-  - intros x. apply cmra_update_updateP, cmra_updateP_id;auto.
-  - intros x y z. rewrite !cmra_update_updateP.
-    intros Hx Hy. intros n mz Hv. apply Hx in Hv as [y' [Heq1 Hy']].
-    rewrite -Heq1 in Hy'. edestruct Hy;eauto.
-Qed.
-Global Instance cmra_update_proper_update :
-  Proper (flip (@cmra_update A t morph) ==> (@cmra_update A t morph) ==> impl) (@cmra_update A t morph).
-Proof.
-  intros x1 x2 Hx y1 y2 Hy ?. etrans; [apply Hx|]. by etrans; [|apply Hy].
-Qed.
-Global Instance cmra_update_flip_proper_update :
-  Proper ((@cmra_update A t morph) ==> flip (@cmra_update A t morph) ==> flip impl) (@cmra_update A t morph).
-Proof.
-  intros x1 x2 Hx y1 y2 Hy ?. etrans; [apply Hx|]. by etrans; [|apply Hy].
-Qed.
+(* (** Updates form a preorder. *) *)
+(* (** We set this rewrite relation's cost above the stdlib's *)
+(*   ([impl], [iff], [eq], ...) and [≡] but below [⊑]. *)
+(*   [eq] (at 100) < [≡] (at 150) < [cmra_update] (at 170) < [⊑] (at 200) *) *)
+(* Global Instance cmra_update_rewrite_relation : *)
+(*   RewriteRelation (@cmra_update A t morph) | 170 := {}. *)
+(* Global Instance cmra_update_preorder : PreOrder (@cmra_update A t morph). *)
+(* Proof. *)
+(*   split. *)
+(*   - intros x. apply cmra_update_updateP, cmra_updateP_id;auto. *)
+(*   - intros x y z. rewrite !cmra_update_updateP. *)
+(*     intros Hx Hy. intros n mz Hv. apply Hx in Hv as [y' [Heq1 Hy']]. *)
+(*     rewrite -Heq1 in Hy'. edestruct Hy;eauto. *)
+(* Qed. *)
+(* Global Instance cmra_update_proper_update : *)
+(*   Proper (flip (@cmra_update A t morph) ==> (@cmra_update A t morph) ==> impl) (@cmra_update A t morph). *)
+(* Proof. *)
+(*   intros x1 x2 Hx y1 y2 Hy ?. etrans; [apply Hx|]. by etrans; [|apply Hy]. *)
+(* Qed. *)
+(* Global Instance cmra_update_flip_proper_update : *)
+(*   Proper ((@cmra_update A t morph) ==> flip (@cmra_update A t morph) ==> flip impl) (@cmra_update A t morph). *)
+(* Proof. *)
+(*   intros x1 x2 Hx y1 y2 Hy ?. etrans; [apply Hx|]. by etrans; [|apply Hy]. *)
+(* Qed. *)
 
 (* Lemma cmra_morphism_option_op : *)
 (*   forall (x : A) (y : option A), t (x ⋅? y) ≡ t x ⋅? (y ≫= t). *)
@@ -105,43 +149,43 @@ Qed.
 (*   by apply cmra_morphism_op. *)
 (* Qed. *)
 
-Lemma cmra_updateP_op (P1 P2 Q : A → Prop) x1 x2 :
-  x1 ~~>:{t} P1 → x2 ~~>:{t} P2 →
-  (∀ y1 y2, P1 (y1) → P2 (y2) → Q (y1 ⋅ y2)) →
-  (∀ x x1 x2, t x ≡ x -> x ≡ x1 ⋅ x2 -> t x1 ≡ x1) ->
-  x1 ⋅ x2 ~~>:{t} Q.
-Proof.
-  intros Hx1 Hx2 Hy Hx n mz [Hv Heq].
-  destruct (Hx1 n (Some (x2 ⋅? mz))) as (y1&?&?&Heq1).
-  { simpl in *. rewrite -cmra_op_opM_assoc//. apply (Hx (x1 ⋅ x2) x1 x2) in Heq =>//. }
-  destruct (Hx2 n (Some (t y1 ⋅? mz))) as (y2&?&Hv2&Heq2).
-  { rewrite /= -cmra_op_opM_assoc (comm _ x2) cmra_op_opM_assoc.
-    apply (Hx (x1 ⋅ x2) x2 x1) in Heq;[|rewrite comm//]. rewrite Heq1. auto. }
-  exists (y1 ⋅ y2). rewrite Heq1 in Hv2.
-  split; try rewrite cmra_morphism_op; last rewrite {1}(comm _ (y1)) cmra_op_opM_assoc; auto.
-  rewrite Heq1 Heq2 //.
-Qed.
-Lemma cmra_updateP_op' (P1 P2 : A → Prop) x1 x2 :
-  x1 ~~>:{t} P1 → x2 ~~>:{t} P2 →
-  (∀ x x1 x2, t x ≡ x -> x ≡ x1 ⋅ x2 -> t x1 ≡ x1) ->
-  x1 ⋅ x2 ~~>:{t} λ y, ∃ y1 y2, y ≡ y1 ⋅ y2 /\ P1 y1 ∧ P2 y2.
-Proof. eauto 10 using cmra_updateP_op. Qed.
-Lemma cmra_update_op x1 x2 y1 y2 :
-  (∀ x x1 x2, t x ≡ x -> x ≡ x1 ⋅ x2 -> t x1 ≡ x1) ->
-  x1 ~~>{t} y1 → x2 ~~>{t} y2 → x1 ⋅ x2 ~~>{t} y1 ⋅ y2.
-Proof.
-  rewrite !cmra_update_updateP'.
-  intros Hop HP1 HP2 n mz [Hv Hx12].
-  destruct (HP1 n (Some (x2 ⋅? mz))) as (y1'&?&?&Heq1);[rewrite /=;auto|].
-  { rewrite /= -cmra_op_opM_assoc. apply (Hop (x1 ⋅ x2) x1 x2) in Hx12;auto. }
-  destruct (HP2 n (Some (y1' ⋅? mz))) as (y2'&?&?&Heq2).
-  { rewrite /= -cmra_op_opM_assoc (comm _ (x2)) cmra_op_opM_assoc.
-    apply (Hop (x1 ⋅ x2) x2 x1) in Hx12;auto. by rewrite comm. }
-  simpl in *. exists (y1' ⋅ y2').
-  rewrite !cmra_morphism_op H H1.
-  repeat split;auto; first rewrite (comm _ (y1')) cmra_op_opM_assoc; auto.
-  rewrite Heq1 Heq2 //.
-Qed.
+(* Lemma cmra_updateP_op (P1 P2 Q : A → Prop) x1 x2 : *)
+(*   x1 ~~>:{t} P1 → x2 ~~>:{t} P2 → *)
+(*   (∀ y1 y2, P1 (y1) → P2 (y2) → Q (y1 ⋅ y2)) → *)
+(*   (∀ x x1 x2, t x ≡ x -> x ≡ x1 ⋅ x2 -> t x1 ≡ x1) -> *)
+(*   x1 ⋅ x2 ~~>:{t} Q. *)
+(* Proof. *)
+(*   intros Hx1 Hx2 Hy Hx n mz [Hv Heq]. *)
+(*   destruct (Hx1 n (Some (x2 ⋅? mz))) as (y1&?&?&Heq1). *)
+(*   { simpl in *. rewrite -cmra_op_opM_assoc//. apply (Hx (x1 ⋅ x2) x1 x2) in Heq =>//. } *)
+(*   destruct (Hx2 n (Some (t y1 ⋅? mz))) as (y2&?&Hv2&Heq2). *)
+(*   { rewrite /= -cmra_op_opM_assoc (comm _ x2) cmra_op_opM_assoc. *)
+(*     apply (Hx (x1 ⋅ x2) x2 x1) in Heq;[|rewrite comm//]. rewrite Heq1. auto. } *)
+(*   exists (y1 ⋅ y2). rewrite Heq1 in Hv2. *)
+(*   split; try rewrite cmra_morphism_op; last rewrite {1}(comm _ (y1)) cmra_op_opM_assoc; auto. *)
+(*   rewrite Heq1 Heq2 //. *)
+(* Qed. *)
+(* Lemma cmra_updateP_op' (P1 P2 : A → Prop) x1 x2 : *)
+(*   x1 ~~>:{t} P1 → x2 ~~>:{t} P2 → *)
+(*   (∀ x x1 x2, t x ≡ x -> x ≡ x1 ⋅ x2 -> t x1 ≡ x1) -> *)
+(*   x1 ⋅ x2 ~~>:{t} λ y, ∃ y1 y2, y ≡ y1 ⋅ y2 /\ P1 y1 ∧ P2 y2. *)
+(* Proof. eauto 10 using cmra_updateP_op. Qed. *)
+(* Lemma cmra_update_op x1 x2 y1 y2 : *)
+(*   (∀ x x1 x2, t x ≡ x -> x ≡ x1 ⋅ x2 -> t x1 ≡ x1) -> *)
+(*   x1 ~~>{t} y1 → x2 ~~>{t} y2 → x1 ⋅ x2 ~~>{t} y1 ⋅ y2. *)
+(* Proof. *)
+(*   rewrite !cmra_update_updateP'. *)
+(*   intros Hop HP1 HP2 n mz [Hv Hx12]. *)
+(*   destruct (HP1 n (Some (x2 ⋅? mz))) as (y1'&?&?&Heq1);[rewrite /=;auto|]. *)
+(*   { rewrite /= -cmra_op_opM_assoc. apply (Hop (x1 ⋅ x2) x1 x2) in Hx12;auto. } *)
+(*   destruct (HP2 n (Some (y1' ⋅? mz))) as (y2'&?&?&Heq2). *)
+(*   { rewrite /= -cmra_op_opM_assoc (comm _ (x2)) cmra_op_opM_assoc. *)
+(*     apply (Hop (x1 ⋅ x2) x2 x1) in Hx12;auto. by rewrite comm. } *)
+(*   simpl in *. exists (y1' ⋅ y2'). *)
+(*   rewrite !cmra_morphism_op H H1. *)
+(*   repeat split;auto; first rewrite (comm _ (y1')) cmra_op_opM_assoc; auto. *)
+(*   rewrite Heq1 Heq2 //. *)
+(* Qed. *)
 
 (* Global Instance cmra_update_op_proper : *)
 (*   Proper ((@cmra_update A t morph) ==> (@cmra_update A t morph) ==> (@cmra_update A t morph)) (op (A:=A)). *)
@@ -158,98 +202,98 @@ Qed.
 (* Lemma cmra_update_included x y : x ≼ y → y ~~>{t} x. *)
 (* Proof. intros [z ->]. apply cmra_update_op_l. Qed. *)
 
-Lemma cmra_update_valid0 x y : (✓{0} x → x ~~>{t} y) → x ~~>{t} y.
-Proof.
-  intros H n mz Hmz. apply H, Hmz.
-  apply (cmra_validN_le n); last lia.
-  destruct mz.
-  - eapply cmra_validN_op_l, Hmz.
-  - apply Hmz.
-Qed.
+(* Lemma cmra_update_valid0 x y : (✓{0} x → x ~~>{t} y) → x ~~>{t} y. *)
+(* Proof. *)
+(*   intros H n mz Hmz. apply H, Hmz. *)
+(*   apply (cmra_validN_le n); last lia. *)
+(*   destruct mz. *)
+(*   - eapply cmra_validN_op_l, Hmz. *)
+(*   - apply Hmz. *)
+(* Qed. *)
 
-(** ** Frame preserving updates for total CMRAs *)
-Section total_updates.
-  Local Set Default Proof Using "Type*".
-  Context `{!CmraTotal A}.
+(* (** ** Frame preserving updates for total CMRAs *) *)
+(* Section total_updates. *)
+(*   Local Set Default Proof Using "Type*". *)
+(*   Context `{!CmraTotal A}. *)
 
-  Lemma cmra_total_updateP x (P : A → Prop) :
-    x ~~>:{t} P ↔ ∀ n z, ✓{n} (x ⋅ z) /\ t x ≡ x → ∃ y, P (y) ∧ ✓{n} (y ⋅ z) /\ t y ≡ y.
-  Proof.
-    split=> Hup; [intros n z ?; apply (Hup n (Some z))|];auto.
-    intros n [z|] [? Heq]; simpl; [by apply Hup|].
-    destruct (Hup n (core (t x))) as (y&?&?&Heq2).
-    - destruct morph. specialize (cmra_morphism_pcore x).
-      rewrite !cmra_pcore_core /= in cmra_morphism_pcore.
-      inversion cmra_morphism_pcore;subst. rewrite -H2.
-      rewrite H2 Heq cmra_core_r //.
-    - eauto using cmra_validN_op_l.
-  Qed.
-  Lemma cmra_total_update x y : x ~~>{t} y ↔ ∀ n z, ✓{n} (x ⋅ z) /\ t x ≡ x → ✓{n} (y ⋅ z) /\ t y ≡ y.
-  Proof. rewrite cmra_update_updateP cmra_total_updateP. split;intros;eauto.
-         edestruct H as [? [-> H']];eauto. Qed.
+(*   Lemma cmra_total_updateP x (P : A → Prop) : *)
+(*     x ~~>:{t} P ↔ ∀ n z, ✓{n} (x ⋅ z) /\ t x ≡ x → ∃ y, P (y) ∧ ✓{n} (y ⋅ z) /\ t y ≡ y. *)
+(*   Proof. *)
+(*     split=> Hup; [intros n z ?; apply (Hup n (Some z))|];auto. *)
+(*     intros n [z|] [? Heq]; simpl; [by apply Hup|]. *)
+(*     destruct (Hup n (core (t x))) as (y&?&?&Heq2). *)
+(*     - destruct morph. specialize (cmra_morphism_pcore x). *)
+(*       rewrite !cmra_pcore_core /= in cmra_morphism_pcore. *)
+(*       inversion cmra_morphism_pcore;subst. rewrite -H2. *)
+(*       rewrite H2 Heq cmra_core_r //. *)
+(*     - eauto using cmra_validN_op_l. *)
+(*   Qed. *)
+(*   Lemma cmra_total_update x y : x ~~>{t} y ↔ ∀ n z, ✓{n} (x ⋅ z) /\ t x ≡ x → ✓{n} (y ⋅ z) /\ t y ≡ y. *)
+(*   Proof. rewrite cmra_update_updateP cmra_total_updateP. split;intros;eauto. *)
+(*          edestruct H as [? [-> H']];eauto. Qed. *)
 
-  Context `{!CmraDiscrete A}.
+(*   Context `{!CmraDiscrete A}. *)
 
-  Lemma cmra_discrete_updateP (x : A) (P : A → Prop) :
-    x ~~>:{t} P ↔ ∀ z, ✓ (x ⋅ z) /\ t x ≡ x → ∃ y, P (y) ∧ ✓ (y ⋅ z) /\ t y ≡ y.
-  Proof.
-    rewrite cmra_total_updateP; setoid_rewrite <-cmra_discrete_valid_iff.
-    naive_solver eauto using O.
-  Qed.
-  Lemma cmra_discrete_update (x y : A) :
-    x ~~>{t} y ↔ ∀ z, ✓ (x ⋅ z) /\ t x ≡ x → ✓ (y ⋅ z) /\ t y ≡ y.
-  Proof.
-    rewrite cmra_total_update; setoid_rewrite <-cmra_discrete_valid_iff.
-    naive_solver eauto using O.
-  Qed.
-End total_updates.
+(*   Lemma cmra_discrete_updateP (x : A) (P : A → Prop) : *)
+(*     x ~~>:{t} P ↔ ∀ z, ✓ (x ⋅ z) /\ t x ≡ x → ∃ y, P (y) ∧ ✓ (y ⋅ z) /\ t y ≡ y. *)
+(*   Proof. *)
+(*     rewrite cmra_total_updateP; setoid_rewrite <-cmra_discrete_valid_iff. *)
+(*     naive_solver eauto using O. *)
+(*   Qed. *)
+(*   Lemma cmra_discrete_update (x y : A) : *)
+(*     x ~~>{t} y ↔ ∀ z, ✓ (x ⋅ z) /\ t x ≡ x → ✓ (y ⋅ z) /\ t y ≡ y. *)
+(*   Proof. *)
+(*     rewrite cmra_total_update; setoid_rewrite <-cmra_discrete_valid_iff. *)
+(*     naive_solver eauto using O. *)
+(*   Qed. *)
+(* End total_updates. *)
 End updates.
 
-(** * Product *)
-Section prod.
-  Context {A B : cmra} (f : B -> B) (t : A -> A) `{morphf: !CmraMorphism f} `{morpht: !CmraMorphism t}.
-  Implicit Types x : A * B.
+(* (** * Product *) *)
+(* Section prod. *)
+(*   Context {A B : cmra} (f : B -> B) (t : A -> A) `{morphf: !CmraMorphism f} `{morpht: !CmraMorphism t}. *)
+(*   Implicit Types x : A * B. *)
 
-  Lemma prod_updateP P1 P2 (Q : A * B → Prop) x :
-    x.1 ~~>:{t} P1 → x.2 ~~>:{f} P2 → (∀ a b, P1 (a) → P2 (b) → Q (a,b)) → x ~~>:{λ x, (t x.1,f x.2)} Q.
-  Proof.
-    intros Hx1 Hx2 HP n mz [[??][??]]; simpl in *.
-    destruct (Hx1 n (fst <$> mz)) as (a&?&?&?); first by destruct mz.
-    destruct (Hx2 n (snd <$> mz)) as (b&?&?&?); first by destruct mz.
-    exists (a,b); repeat split; destruct mz; auto.
-  Qed.
-  Lemma prod_updateP' P1 P2 x :
-    x.1 ~~>:{t} P1 → x.2 ~~>:{f} P2 → x ~~>:{λ x, (t x.1,f x.2)} λ y, P1 y.1 ∧ P2 y.2.
-  Proof. eauto using prod_updateP. Qed.
-  Lemma prod_update x y : x.1 ~~>{t} y.1 → x.2 ~~>{f} y.2 → x ~~>{λ x, (t x.1, f x.2)} y.
-  Proof.
-    rewrite !cmra_update_updateP.
-    destruct x, y; simpl.
-    intros. eapply prod_updateP;eauto.
-    intros a b -> -> =>//.
-  Qed.
-End prod.
+(*   Lemma prod_updateP P1 P2 (Q : A * B → Prop) x : *)
+(*     x.1 ~~>:{t} P1 → x.2 ~~>:{f} P2 → (∀ a b, P1 (a) → P2 (b) → Q (a,b)) → x ~~>:{λ x, (t x.1,f x.2)} Q. *)
+(*   Proof. *)
+(*     intros Hx1 Hx2 HP n mz [[??][??]]; simpl in *. *)
+(*     destruct (Hx1 n (fst <$> mz)) as (a&?&?&?); first by destruct mz. *)
+(*     destruct (Hx2 n (snd <$> mz)) as (b&?&?&?); first by destruct mz. *)
+(*     exists (a,b); repeat split; destruct mz; auto. *)
+(*   Qed. *)
+(*   Lemma prod_updateP' P1 P2 x : *)
+(*     x.1 ~~>:{t} P1 → x.2 ~~>:{f} P2 → x ~~>:{λ x, (t x.1,f x.2)} λ y, P1 y.1 ∧ P2 y.2. *)
+(*   Proof. eauto using prod_updateP. Qed. *)
+(*   Lemma prod_update x y : x.1 ~~>{t} y.1 → x.2 ~~>{f} y.2 → x ~~>{λ x, (t x.1, f x.2)} y. *)
+(*   Proof. *)
+(*     rewrite !cmra_update_updateP. *)
+(*     destruct x, y; simpl. *)
+(*     intros. eapply prod_updateP;eauto. *)
+(*     intros a b -> -> =>//. *)
+(*   Qed. *)
+(* End prod. *)
 
-Local Infix "≫=" := (λ mz t, (mz ≫= (λ x, Some (t x)))).
+(* Local Infix "≫=" := (λ mz t, (mz ≫= (λ x, Some (t x)))). *)
 
-(** * Option *)
-Section option.
-  Context {A : cmra} (t : A -> A) `{morph: !CmraMorphism t}.
-  Implicit Types x y : A.
+(* (** * Option *) *)
+(* Section option. *)
+(*   Context {A : cmra} (t : A -> A) `{morph: !CmraMorphism t}. *)
+(*   Implicit Types x y : A. *)
 
-  Lemma option_updateP (P : A → Prop) (Q : option A → Prop) x :
-    x ~~>:{t} P → (∀ y, P (y) → Q (Some (y))) → Some x ~~>:{λ (x : option A), x ≫= t} Q.
-  Proof.
-    intros Hx Hy. intros n mz Hn. destruct mz.
-    { simpl in *. rewrite Some_op_opM Some_validN in Hn. destruct Hn as [Hv Hn].
-      inversion Hn;subst. edestruct Hx as [? [? [? ?]]];eauto.
-      eexists (Some x0). rewrite Some_op_opM /=. repeat split;auto. f_equiv. auto. }
-    simpl in *. rewrite Some_validN in Hn. destruct Hn as [Hv Hn].
-    inversion Hn;subst.
-    edestruct (Hx n None) as [? [? [? ?]]];auto.
-    eexists (Some _). simpl. repeat split; eauto. f_equiv. auto.
-  Qed.
-  Lemma option_update x y : x ~~>{t} y → Some x ~~>{λ (x : option A), x ≫= t} Some y.
-  Proof. rewrite !cmra_update_updateP. intros. eapply option_updateP;eauto.
-         intros. simpl. f_equiv;auto. Qed.
-End option.
+(*   Lemma option_updateP (P : A → Prop) (Q : option A → Prop) x : *)
+(*     x ~~>:{t} P → (∀ y, P (y) → Q (Some (y))) → Some x ~~>:{λ (x : option A), x ≫= t} Q. *)
+(*   Proof. *)
+(*     intros Hx Hy. intros n mz Hn. destruct mz. *)
+(*     { simpl in *. rewrite Some_op_opM Some_validN in Hn. destruct Hn as [Hv Hn]. *)
+(*       inversion Hn;subst. edestruct Hx as [? [? [? ?]]];eauto. *)
+(*       eexists (Some x0). rewrite Some_op_opM /=. repeat split;auto. f_equiv. auto. } *)
+(*     simpl in *. rewrite Some_validN in Hn. destruct Hn as [Hv Hn]. *)
+(*     inversion Hn;subst. *)
+(*     edestruct (Hx n None) as [? [? [? ?]]];auto. *)
+(*     eexists (Some _). simpl. repeat split; eauto. f_equiv. auto. *)
+(*   Qed. *)
+(*   Lemma option_update x y : x ~~>{t} y → Some x ~~>{λ (x : option A), x ≫= t} Some y. *)
+(*   Proof. rewrite !cmra_update_updateP. intros. eapply option_updateP;eauto. *)
+(*          intros. simpl. f_equiv;auto. Qed. *)
+(* End option. *)
